Generalize the trusted bridge

src/trusted_code/k8s_io/client_go/gentype.v
@@ -1,8 +1,10 @@
 From New.golang Require Import defn.
 Require Import New.code.context.
 Require Import New.code.kubernetes_model.apimodel.
+Require Import New.code.k8s_io.api.apps.v1.
 Require Import New.code.k8s_io.api.core.v1.
 Require Import New.code.k8s_io.apimachinery.pkg.apis.meta.v1.
+Module api_apps_v1 := code.k8s_io.api.apps.v1.v1.
 Module api_core_v1 := code.k8s_io.api.core.v1.v1.
 Module meta_v1 := code.k8s_io.apimachinery.pkg.apis.meta.v1.v1.
 
@@ -18,33 +20,68 @@ Definition clientType (T : go.type) : go.type :=
    func (c *Client[T]) Create(ctx context.Context, obj T, opts metav1.CreateOptions) (T, error) {
        _ = ctx
        _ = opts
-       type podPointer = *corev1.Pod
-       typed := any(obj).(podPointer)
-       created, err := apimodel.ModelState.PodCreate(c.namespace, typed)
-       return any(created).(T), err
+       switch typed := any(obj).(type) {
+       case *corev1.Pod:
+           created, err := apimodel.ModelState.PodCreate(c.namespace, typed)
+           return any(created).(T), err
+       case *appsv1.ReplicaSet:
+           created, err := apimodel.ModelState.ReplicaSetCreate(c.namespace, typed)
+           return any(created).(T), err
+       case *corev1.PersistentVolumeClaim:
+           created, err := apimodel.ModelState.PersistentVolumeClaimCreate(c.namespace, typed)
+           return any(created).(T), err
+       case *appsv1.StatefulSet:
+           created, err := apimodel.ModelState.StatefulSetCreate(c.namespace, typed)
+           return any(created).(T), err
+       default:
+           panic("unsupported Kubernetes object type")
+       }
    }
 *)
-Definition Client__Createⁱᵐᵖˡ (T : go.type) : val :=
+Definition clientCreate (T objectType : go.type) (method : go_string) : val :=
   λ: "c" "ctx" "obj" "opts",
     exception_do (let: "c" := (GoAlloc (go.PointerType (clientType T)) "c") in
     let: "obj" := (GoAlloc T "obj") in
     let: "namespace" := (GoAlloc go.string (![go.string] (StructFieldRef (clientType T) "namespace"%go (![go.PointerType (clientType T)] "c")))) in
-    let: "typed" := (GoAlloc (go.PointerType api_core_v1.Pod)
-      (TypeAssert (go.PointerType api_core_v1.Pod) (Convert T go.any (![T] "obj")))) in
+    let: "typed" := (GoAlloc objectType (TypeAssert objectType (Convert T go.any (![T] "obj")))) in
     let: ("$ret0", "$ret1") := (let: "$a0" := (![go.string] "namespace") in
-    let: "$a1" := (![go.PointerType api_core_v1.Pod] "typed") in
-    (MethodResolve (go.PointerType apimodel.State) "PodCreate"%go
+    let: "$a1" := (![objectType] "typed") in
+    (MethodResolve (go.PointerType apimodel.State) method
       (![go.PointerType apimodel.State] (GlobalVarAddr apimodel.ModelState #()))) "$a0" "$a1") in
-    return: (TypeAssert T (Convert (go.PointerType api_core_v1.Pod) go.any "$ret0"), "$ret1")).
+    return: (TypeAssert T (Convert objectType go.any "$ret0"), "$ret1")).
+
+Definition Client__Createⁱᵐᵖˡ (T : go.type) : val :=
+  if decide (T = go.PointerType api_core_v1.Pod) then
+    clientCreate T (go.PointerType api_core_v1.Pod) "PodCreate"%go
+  else if decide (T = go.PointerType api_apps_v1.ReplicaSet) then
+    clientCreate T (go.PointerType api_apps_v1.ReplicaSet) "ReplicaSetCreate"%go
+  else if decide (T = go.PointerType api_core_v1.PersistentVolumeClaim) then
+    clientCreate T (go.PointerType api_core_v1.PersistentVolumeClaim) "PersistentVolumeClaimCreate"%go
+  else if decide (T = go.PointerType api_apps_v1.StatefulSet) then
+    clientCreate T (go.PointerType api_apps_v1.StatefulSet) "StatefulSetCreate"%go
+  else
+    (λ: "c" "ctx" "obj" "opts", Panic "unsupported Kubernetes object type")%V.
 
 (* Trusted Go equivalent:
 
    func (c *Client[T]) Delete(ctx context.Context, name string, opts metav1.DeleteOptions) error {
        _ = ctx
-       return apimodel.ModelState.PodDelete(c.namespace, name, opts)
+       var zero T
+       switch any(zero).(type) {
+       case *corev1.Pod:
+           return apimodel.ModelState.PodDelete(c.namespace, name, opts)
+       case *appsv1.ReplicaSet:
+           return apimodel.ModelState.ReplicaSetDelete(c.namespace, name, opts)
+       case *corev1.PersistentVolumeClaim:
+           return apimodel.ModelState.PersistentVolumeClaimDelete(c.namespace, name, opts)
+       case *appsv1.StatefulSet:
+           return apimodel.ModelState.StatefulSetDelete(c.namespace, name, opts)
+       default:
+           panic("unsupported Kubernetes object type")
+       }
    }
 *)
-Definition Client__Deleteⁱᵐᵖˡ (T : go.type) : val :=
+Definition clientDelete (T : go.type) (method : go_string) : val :=
   λ: "c" "ctx" "name" "opts",
     exception_do (let: "c" := (GoAlloc (go.PointerType (clientType T)) "c") in
     let: "opts" := (GoAlloc meta_v1.DeleteOptions "opts") in
@@ -53,8 +90,20 @@ Definition Client__Deleteⁱᵐᵖˡ (T : go.type) : val :=
     return: (let: "$a0" := (![go.string] "namespace") in
     let: "$a1" := (![go.string] "name") in
     let: "$a2" := (![meta_v1.DeleteOptions] "opts") in
-    (MethodResolve (go.PointerType apimodel.State) "PodDelete"%go
+    (MethodResolve (go.PointerType apimodel.State) method
       (![go.PointerType apimodel.State] (GlobalVarAddr apimodel.ModelState #()))) "$a0" "$a1" "$a2")).
+
+Definition Client__Deleteⁱᵐᵖˡ (T : go.type) : val :=
+  if decide (T = go.PointerType api_core_v1.Pod) then
+    clientDelete T "PodDelete"%go
+  else if decide (T = go.PointerType api_apps_v1.ReplicaSet) then
+    clientDelete T "ReplicaSetDelete"%go
+  else if decide (T = go.PointerType api_core_v1.PersistentVolumeClaim) then
+    clientDelete T "PersistentVolumeClaimDelete"%go
+  else if decide (T = go.PointerType api_apps_v1.StatefulSet) then
+    clientDelete T "StatefulSetDelete"%go
+  else
+    (λ: "c" "ctx" "name" "opts", Panic "unsupported Kubernetes object type")%V.
 
 End code.
 End gentype.
